\documentclass{article}
\begin{document}
\begin{eqnarray*}
\mathrm{bar}&=&0\\
\tau_{{\mathrm{bar}}}&=&0\\
\mathrm{foo}_{1}&=&0\\
d&=&0\\
c&=&0\\
\mathrm{bar}_{2^{3}}&=&0\\
a&=&0\\
A&=&0\\
\mathrm{foo}&=&\mathrm{bar}\\
\mathrm{Repay}&=&\frac{\mathrm{foo}+\tau_{{\mathrm{bar}}}}{\mathrm{Loans}+ t }\\
\mathrm{catching}&=&\exp\left(\left(\mathrm{Loans}+ t -\left(\mathrm{foo}+\tau_{{\mathrm{bar}}}\right)\right)\times b\right)\\
F(0)&=&0\\
\frac{ d F}{dt} &=&\mathrm{foo}\times  t \\
\mathrm{Loans}(0)&=&0\\
\frac{ d \mathrm{Loans}}{dt} &=&A+\mathrm{Repay}-\mathrm{catching}\\
b(0)&=&0\\
\frac{ d b}{dt} &=&\mathrm{catching}-\mathrm{Repay}\\
\mathrm{fooey}(0)&=&0\\
\frac{ d \mathrm{fooey}}{dt} &=&\left(a+b\right)^{\log_{d}\left(c\right)}\\
\mathrm{int}(0)&=&0\\
\frac{ d \mathrm{int}}{dt} &=&\tanh\left(\cosh\left(\sinh\left(\tan\left(\cos\left(\sin\left(\ln\left(\sqrt{ t }\right)\right)\right)\right)\right)\right)\right)\\
\mathrm{int1}(0)&=&0\\
\frac{ d \mathrm{int1}}{dt} &=&\arctan\left(\arccos\left(\arcsin\left( t \right)\right)\right)\\
\end{eqnarray*}
\end{document}
